Update keyring traces with Materials refactor

src/SDK/Keyring/Defs.dfy
@@ -9,6 +9,30 @@ module KeyringDefs {
   import Materials
   import AlgorithmSuite
 
+  // TODO Seems a bit strange to have this defined here but ValidDataKeyMaterials elsewhere, however this is defining logic
+  // specific to keyrings so it might seem misplaced in Materials.dfy
+  // TODO 'res' is already a common name for the out param, so naming this Result might be overloading the term
+  datatype OnDecryptResult = OnDecryptResult(algorithmSuiteID: AlgorithmSuite.ID,
+                                             plaintextDataKey: seq<uint8>,
+                                             keyringTrace: seq<Materials.KeyringTraceEntry>) // TODO does it make sense to define this as a sequence when we are requiring only one for now?
+  {
+    predicate Valid() {
+      && algorithmSuiteID.ValidPlaintextDataKey(plaintextDataKey)
+      && (forall trace :: trace in keyringTrace ==> trace.flags <= Materials.ValidDecryptionMaterialFlags)
+      && |keyringTrace| == 1 && Materials.TraceHasDecryptFlag(keyringTrace[0])
+    }
+
+    static function method ValidWitness(): OnDecryptResult {
+      var pdk := seq(32, i => 0);
+      var trace := Materials.KeyringTraceEntry([], [], {Materials.DECRYPTED_DATA_KEY});
+      var r := OnDecryptResult(AlgorithmSuite.AES_256_GCM_IV12_TAG16_HKDF_SHA384_ECDSA_P384,
+                      pdk, [trace]);
+      r
+    }
+  }
+
+  type ValidOnDecryptResult = i: OnDecryptResult | i.Valid() witness OnDecryptResult.ValidWitness()
+
   trait {:termination false} Keyring {
     ghost var Repr : set<object>
     predicate Valid() reads this, Repr
@@ -20,20 +44,22 @@ module KeyringDefs {
       requires plaintextDataKey.Some? ==> algorithmSuiteID.ValidPlaintextDataKey(plaintextDataKey.get)
       ensures Valid()
       ensures res.Success? && res.value.Some? ==> 
-          algorithmSuiteID == res.value.get.algorithmSuiteID
+        algorithmSuiteID == res.value.get.algorithmSuiteID
       ensures res.Success? && res.value.Some? && plaintextDataKey.Some? ==> 
-          plaintextDataKey.get == res.value.get.plaintextDataKey
-      // TODO: keyring trace GENERATED_DATA_KEY flag assurance
-      // TODO: keyring trace ENCRYPTED_DATA_KEY flag assurance
+        plaintextDataKey.get == res.value.get.plaintextDataKey
+      // TODO: Is there any way we can move the below logic into the dataKeyMaterials itself? Or does that not make sense functionally?
+      ensures res.Success? && res.value.Some? && plaintextDataKey.None? ==>
+        var generateTraces := Filter(res.value.get.keyringTrace, Materials.TraceHasGenerateFlag);
+        |generateTraces| == 1
+      ensures res.Success? && res.value.Some? && plaintextDataKey.Some? ==>
+        var generateTraces := Filter(res.value.get.keyringTrace, Materials.TraceHasGenerateFlag);
+        |generateTraces| == 0
 
     method OnDecrypt(algorithmSuiteID: AlgorithmSuite.ID,
                      encryptionContext: Materials.EncryptionContext,
-                     edks: seq<Materials.EncryptedDataKey>) returns (res: Result<Option<Materials.OnDecryptResult>>)
+                     edks: seq<Materials.EncryptedDataKey>) returns (res: Result<Option<ValidOnDecryptResult>>)
       requires Valid()
       ensures Valid()
       ensures |edks| == 0 ==> res.Success? && res.value.None?
-      ensures res.Success? && res.value.Some? ==> 
-          algorithmSuiteID.ValidPlaintextDataKey(res.value.get)
-      // TODO: keyring trace DECRYPTED_DATA_KEY flag assurance
   }
 }
