src/SDK/CMM/DefaultCMM.dfy
@@ -93,12 +93,12 @@ module DefaultCMMDef {
         vkey := Some(base64Decoded);
       }
 
-      var dm :- kr.OnDecrypt(alg_id, enc_ctx, edks);
-      if dm.None? {
+      var onDecryptResult :- kr.OnDecrypt(alg_id, enc_ctx, edks);
+      if onDecryptResult.None? {
         return Failure("Could not get materials required for decryption.");
       }
 
-      return Success(Materials.DecryptionMaterials(alg_id, enc_ctx, dm.get, vkey));
+      return Success(Materials.DecryptionMaterials(alg_id, enc_ctx, onDecryptResult.get.plaintextDataKey, vkey, onDecryptResult.get.keyringTrace));
     }
   }
 }
